\documentclass[12pt]{article}
\usepackage[a4paper, margin=1.25cm, bottom=2cm]{geometry}

\title{\textbf{CS1231 - 1 - Logic}}
\date{}

\setlength{\parindent}{0cm}
\setlength{\itemsep}{0cm}
\usepackage{graphicx}
\usepackage{mdwlist}
\usepackage{setspace}
\usepackage{color, soul}

\begin{document}

\maketitle
\begin{spacing}{1.5}

\section{Proofs}

\begin{itemize*}
	\item \hl{Direct}
	\item Equivalence (contrapositive, $\neg p \Rightarrow \neg q, p \Rightarrow q$)
	\item Exhaustion (by cases)
	\item Construction
	\item \hl{Counter Example}
	\item \hl{Contradiction}
	\item Contrapositive
	\item \hl{Induction} (Base case, induction hypothesis)
	\item \hl{Combinatorial}
\end{itemize*}

\section{Propositional Logic}

\begin{itemize*}
	\item Negation ($\neg$)
	\item Conjunction/And ($\wedge$)
	\item Disjunction/Or ($\vee$)
	\item Exclusive disjunction/XOR ($\bigoplus$)
	\item Conditional/If-Then/Implies ($\Rightarrow$)
		\begin{itemize*}
		    \item $p \Rightarrow q$
	    		\begin{itemize}
			        \item $p$ - premise
			        \item $q$ - consequence
		        \end{itemize}
		    \item Converse (of $p \Rightarrow q$ is $q \Rightarrow p$)
		    \item Contrapositive (of $p \Rightarrow q$ is $\neg p \Rightarrow \neg q$)
		    \item[]
				\begin{tabular}{ll | l}
					p & q & $p \Rightarrow q$ \\
					\hline
					0 & 0 & 1 \\
					0 & 1 & 1 \\
					1 & 0 & 0 \\
					1 & 1 & 1 
				\end{tabular}
    	\end{itemize*}
	\item Bi-conditional ($\Leftrightarrow$)
		\begin{quote}
			\begin{tabular}{ll | l}
				p & q & $p \Leftrightarrow q$ \\
				\hline
				0 & 0 & 1 \\
				0 & 1 & 0 \\
				1 & 0 & 0 \\
				1 & 1 & 1 
			\end{tabular}
		\end{quote}
		
	\item True ($\top$)
	\item False ($\perp$)
\end{itemize*}

\subsection{Precedence (High to low)} 

$\neg \qquad \bigoplus \qquad \vee \qquad \wedge \qquad \Rightarrow \qquad \Leftrightarrow$

\subsection{Demorgan's law (Negation of AND/OR)}

$~(p \vee q) \equiv ~p \wedge ~q, \qquad ~(p \wedge q) \equiv ~p \vee ~q$

\vspace{0.6cm}

\begin{tabular}{cc | cc | ccc | ccc}
p & q & $\neg p$ & $\neg q$ & $p \vee q$ & $\neg (p \vee q)$ & $\neg p \wedge \neg q$ & $p \wedge q$ & $\neg (p \wedge q)$ & $\neg p \vee \neg q$ \\
\hline 
0 & 0 & 1 & 1 & 0 & 1 & 1 & 0 & 1 & 1 \\ 
0 & 1 & 1 & 0 & 1 & 0 & 0 & 0 & 1 & 1 \\
1 & 0 & 0 & 1 & 1 & 0 & 0 & 0 & 1 & 1 \\
1 & 1 & 0 & 0 & 1 & 0 & 0 & 1 & 0 & 1 \\
\end{tabular}

\section{Predicate Logic}

\texttt{odd(n)} $\Rightarrow$ n is odd

\texttt{odd('$\times$'('$+$'(3, 2), 5))} $\Rightarrow$ $(3+2) \times 5$ is odd

\subsection{Quantifiers}

\begin{tabular}{l | l}
$\forall$ & For all \\
$\exists$ & There exists
\end{tabular}

$F[t/X] \Rightarrow $ is Formula, $F$, where we substitude $X$ with $t$

\section{Post Systems}

\begin{itemize*}
	\item Alphabet/symbols $\rightarrow$ words
	\item Axioms: collection of words
	\item Inferance rules: $P_1, ... , P_n \vdash P_{n+1} $, where $P_i$ are word patterns containing variables
	\item $A \vdash B$: A proves B
\end{itemize*}

\underline{Example}: 

Given:

\begin{itemize*}
	\item Alphabet: ${A, B, C}$
	\item Axioms: $A, BC$
	\item Rules: $BX \vdash XX$, $A,XX \vdash XBA$
\end{itemize*}

Prove CBA

\begin{itemize*}
	\item BC (Axiom)
	\item CC ($BX \vdash XX$)
	\item A, Axiom
	\item $A, CC \vdash CBA$
	\item CBA
\end{itemize*}

Assume BB. Then prove BABA

\begin{itemize*}
	\item BB (Assumption)
		\begin{itemize*}
			\item A (Axiom)
			\item $A, BB \vdash BBA (A,XX \vdash XBA)$
			\item $BBA \vdash BABA (BX \vdash XX)$
		\end{itemize*}
\end{itemize*}

Consider discharge rule $(XX \vdash XAXA) \vdash XA$

\begin{itemize*}
	\item ... continue from above ... $BB \vdash BABA$
	\item $(BB \vdash BABA) \vdash BA ((XX \vdash XAXA) \vdash XA)$
\end{itemize*}

\section{Natural Deduction}

\begin{itemize*}
	\item $A, B \vdash A \wedge B$ \qquad (Conjuction introducation)
	\item $(A \wedge B) \vdash A, \quad (A \wedge B) \vdash B$ \qquad (Conjunction elimination)
	\item $A \vdash (A \vee B), \quad B \vdash (A \vee B)$ \qquad (Disjuction introduction)
	\item $(A \Rightarrow X, B \Rightarrow X, A \vee B) \vdash X$ \qquad (Disjunction elimination)
	\item $\neg \neg A = A$ \qquad (Double negation)
	\item $(A \Rightarrow (B \wedge \neg B)) \vdash \neg A$ \qquad (Negation introduction)
	\item $(A \vdash B) \vdash (A \Rightarrow B)$ \qquad (Implication introduction)
\end{itemize*}

\subsection{Others}

\textbf{$(A \wedge B) \vdash (B \wedge A) $, Conjunction Commutativity}

\begin{enumerate*}
	\item $A \wedge B$ \qquad (Premise)
	\item A \qquad ($A \wedge B \vdash A)$
	\item B \qquad ( $A \wedge B \vdash B)$
	\item $B \vdash A \qquad (B, A \vdash B \wedge A)$ 
\end{enumerate*}

\textbf{$A \vdash \neg \neg A$, Double negation introduction}

\begin{enumerate*}
	\item $F_1$, (premise)
	\item Assume $\neg F_1$
		\begin{enumerate*}
			\item $F_1 \wedge \neg F_1$, (conjuction introduction with 1 \& 2)
		\end{enumerate*}
	\item $\neg F_1 \Rightarrow F_1 \wedge \neg F_1$, (implication introduction of 2 \& 2.1)
	\item $\neg \neg F_1$, (negation introduction with 3)
\end{enumerate*}

\textbf{$F_1, \neg F_1 \vdash F_2$, Negation elimination}

\textbf{$F_1, F_1 \Rightarrow F_2 \vdash F_2$, Implication Elimination/Modus Ponens}

\begin{enumerate*}
	\item $F_1$, (premise)
	\item $F_1 \Rightarrow F_2$, (premise)
	\item $F_1 \vee F_1$, (disjunction introduction with 1 \& 1)
	\item $F_2$ by disjunction elimination with 3, 2, 2
\end{enumerate*}

\section{Propositional Calculus}

\begin{itemize*}
	\item Interpretation (I) is mapping of propositions to truth values
		\begin{itemize*}
			\item \textbf{Logical Consequence ($vDash$)}
		\end{itemize*}
\end{itemize*} 


\section{Boolean Algebra}

\begin{itemize*}
	\item \textbf{Identity of $\times$}: $x \times 1 - x$
	\item \textbf{Identity of plus}: $x + 0 = x$
	\item \textbf{Complementation of $\times$}: $x \times \overline{x} = 0$
	\item \textbf{Complementation of +}: $x + \overline{x} = 1$
	\item \textbf{Associativity of $\times$}: $x \times (y \times z) = (x \times y) \times z$
	\item \textbf{Associativity of +}: $x + (y + z) = (x + y) + z$
	\item \textbf{Commutativity of $\times$}: $x \times y = y \times z$
	\item \textbf{Commutativity of +}: $x + y = y + z$
	\item \textbf{Distributivity of $\times$ over +}: $x \times (y + z) = (x \times y) + (x \times z)$
	\item \textbf{Distributivity of + over $\times$}: $x + (y \times z) = (x + y) \times (x + z)$
	\item \textbf{Idempotence of $\times$}: $x \times x = x$
	\item \textbf{Idempotence of +}: $x + x = x$
	\item \textbf{Annihilator of $\times$}: $x \times 0 = 0$
	\item \textbf{Annihilator of +}: $x + 1 = 1$
	\item \textbf{Absorbsion of $\times$}: $x \times (x + y) = x$
	\item \textbf{Absorption of +}: $x + (x \times y) = x$
	\item \textbf{Double negation}: $\overline{\overline{x}} = x$
	\item \textbf{De Morgan's Law for $\times$}: $\overline{x \times y} = \overline{x} + \overline{y}$
	\item \textbf{De Morgan's Law for +}: $\overline{x + y} = \overline{x} \times \overline{y}$
\end{itemize*}

\end{spacing}
\end{document}